Imp.no_whiles_eqv implementation

Imp.v
@@ -1697,13 +1697,66 @@ Fixpoint no_whiles (c : com) : bool :=
     while loops.  Then prove its equivalence with [no_whiles]. *)
 
 Inductive no_whilesR: com -> Prop :=
- (* FILL IN HERE *)
+  | no_whilesR_skip : no_whilesR <{ skip }>
+  | no_whilesR_asgn (x : string) (a : aexp) : no_whilesR <{ x := a }>
+  | no_whilesR_seq (c1 c2 : com) (H_c1: no_whilesR c1) (H_c2: no_whilesR c2) :
+      no_whilesR <{ c1 ; c2 }>
+  | no_whilesR_if (b: bexp) (ct cf : com)
+    (H_ct: no_whilesR ct) (H_cf: no_whilesR cf) :
+      no_whilesR <{ if b then ct else cf end }>
 .
+
+Theorem n_while_eqv_fixpoint_to_R:
+  forall c, no_whiles c = true -> no_whilesR c.
+Proof.
+  intros c H_no_whiles. induction c.
+  - constructor.
+  - constructor.
+  - simpl in H_no_whiles. constructor.
+    + apply IHc1. destruct (no_whiles c1) eqn:H_no_whiles_c1.
+      * reflexivity.
+      * discriminate.
+    + apply IHc2. destruct (no_whiles c2) eqn:H_no_whiles_c2.
+      * reflexivity.
+      * rewrite andb_false_r in H_no_whiles. discriminate.
+  - simpl in H_no_whiles. constructor.
+    + apply IHc1. destruct (no_whiles c1) eqn:H_no_whiles_c1.
+      * reflexivity.
+      * discriminate.
+    + apply IHc2. destruct (no_whiles c2) eqn:H_no_whiles_c2.
+      * reflexivity.
+      * rewrite andb_false_r in H_no_whiles. discriminate.
+  - simpl in H_no_whiles. discriminate.
+Qed.
+
+Theorem n_while_eqv_R_to_fixpoint:
+  forall c, no_whilesR c -> no_whiles c = true.
+Proof.
+  intros c H_no_whilesR.
+  induction H_no_whilesR as [
+    (* skip *)
+    (* assignment *)
+    | x a
+    (* seq *)
+    | c1 c2 Hc1 IHc1 Hc2 IHc2 
+    (* if *)
+    | b ct cf Hct IHct Hcf IHcf
+  ].
+  - reflexivity.
+  - reflexivity.
+  - simpl. rewrite -> IHc1. rewrite -> IHc2.
+    reflexivity.
+  - simpl. rewrite -> IHct. rewrite -> IHcf.
+    reflexivity.
+Qed.
 
 Theorem no_whiles_eqv:
   forall c, no_whiles c = true <-> no_whilesR c.
 Proof.
-  (* FILL IN HERE *) Admitted.
+  split.
+  - apply n_while_eqv_fixpoint_to_R.
+  - apply n_while_eqv_R_to_fixpoint.
+Qed.
 (** [] *)
 
 (** **** Exercise: 4 stars, standard (no_whiles_terminating)
